Java/src/Logic/IsMarshallable.v
@@ -1,0 +1,112 @@
+Require Import Program  Heap ProtocolLogic AssertionLogic OperationalSemantics SpecLogic Util.
+Require Import MapInterface MapFacts.
+Require Import SepAlg SepAlgInsts ILInsts ILogic ILEmbed ILEmbedTac ILQuantTac OpenILogic
+               SepAlgMap UUSepAlg Open Subst Stack Lang SemCmd HeapArr ST SemCmdRules BILogic BILInsts.
+
+
+Local Transparent ILPre_Ops.
+Local Transparent ILPreFrm_pred.
+Local Transparent EmbedSasnPureOp.
+Local Transparent EmbedILFunOp.
+Local Transparent EmbedAsnPropOp.
+Local Transparent ILPre_Ops.
+Local Transparent EmbedILPreDropOp.
+Local Transparent EmbedILPreOp.
+Local Transparent MapSepAlgOps.
+Local Transparent ILFun_Ops.
+Local Transparent EmbedILFunDropOp.
+Local Transparent EmbedILFunOp.
+Local Transparent SepAlgOps_prod.
+
+Local Transparent EmbedILPreDropOp.
+Local Transparent EmbedILFunDropOp.
+Local Transparent EmbedPSasnPropOp.
+Local Transparent EmbedAsnPropOp.
+Local Transparent BILOperatorsPSasn.
+Local Transparent BILFun_Ops.
+Local Transparent BILOperatorsAsn.
+
+Lemma pointsto_IsMarshallable (v : var) (f : field) (e : expr):
+  Exists C, field_exists C f /\\ embed (@land sasn _ (v ::: C) (`pointsto v/V `f e))
+  |--
+  isMarshallable v (`pointsto v/V `f e). 
+Proof.
+  intros s PM STs Pr n h [C [Hfield [Htypeof Hpointsto]]].
+  simpl in Htypeof; simpl in Hfield; simpl in Hpointsto; unfold var_expr in Hpointsto.
+  unfold typeof, liftn, lift, var_expr in Htypeof; simpl in Htypeof.
+  destruct Htypeof as [p [Href Hclass]].
+  destruct Hfield as [fields [Hfields Hisfield]].
+  destruct p as [pos cls]; simpl in Hclass; rewrite Hclass in *; clear Hclass.
+    
+  unfold liftn, lift, var_expr; simpl.
+  intros.
+  split; [apply Hpointsto |].
+  induction H; [
+  	rewrite Vint in Href |
+   	rewrite Vbool in Href |
+   	rewrite Vptr in Href
+  ]; inversion Href; subst.
+  inversion H1; subst; simpl; clear H1 Href.
+  exists (remove ((pos, C), f) (get_heap_ptr m)).
+    
+  apply sa_mul_swapL; [apply sa_mulC; apply uusa_unit; apply empty_1 |].
+  (* Make Hisfield talk about field0 *)
+  assert (SS.Equal fields fields0) by (eapply field_lookup_function_sub; eassumption).
+  rewrite H0 in Hisfield; clear H0.
+  (* And then use Mhere, now that we have the field0 evidence *)
+  apply Mhere; assumption.
+Qed.
+
+Lemma pointsto_IsMarshallable_2 (v : var) (f : field) (e : expr) (Q : sasn):
+  Exists C, field_exists C f /\\ embed (@land sasn _ (v ::: C) (`pointsto v/V `f e)) ** isMarshallable v Q
+  |--
+  isMarshallable v (@land sasn _ (`pointsto v/V `f e) Q). 
+Proof.
+  intros s PM STs Pr n h [C [Hfield [h1 [h2 [Hcompose [[Htypeof Hpointsto] HIM]]]]]].
+  simpl in Htypeof; simpl in Hfield; simpl in Hpointsto; unfold var_expr in Hpointsto.
+  unfold typeof, liftn, lift, var_expr in Htypeof; simpl in Htypeof.
+  unfold liftn, lift in Hpointsto; simpl in Hpointsto.
+  destruct Htypeof as [p [Href Hclass]].
+  destruct Hfield as [fields [Hfields Hisfield]].
+  destruct p as [pos cls]; simpl in Hclass; rewrite Hclass in *; clear Hclass.
+  rewrite Href in *. simpl in *.
+  
+  unfold liftn, lift, var_expr; simpl; unfold id.
+  intros; simpl.
+  (* Use the introduced info to specialize HIM with *)
+  (* TODO: This needs to not use h', but something without (pos, C, f) in it) *)
+  assert (subheap h2 h') by (transitivity h; [ exists h1; apply sa_mulC; assumption | assumption ]).
+  specialize (HIM _ _ _ k' H0 Hsp H); clear H0.
+  (* Prove that the pointer is present in the marshalling *) 
+  assert (MapsTo (pos, C, f) (e s) (get_heap_ptr m)). {
+    inversion H; [
+      rewrite Vint in Href |
+      rewrite Vbool in Href |
+      rewrite Vptr in Href
+    ]; inversion Href. 
+    rewrite Vclass in H2; inversion H2; subst.
+    assert (SS.Equal fields fields0) by (eapply field_lookup_function_sub; eassumption).
+    eapply Mhere; rewrite <- H0; assumption.
+  }
+  (* Setup the two disjoint heaps for the goal, m1 and m2 *
+  remember (mkheap (add (pos, C, f) (e s) (empty _)) (empty _)) as m1.
+  remember (mkheap (remove (pos, C ,f) (get_heap_ptr m)) (get_heap_arr m)) as m2.
+  assert (sa_mul m1 m2 m). {
+    rewrite Heqm1, Heqm2.
+    apply split_heap; simpl.
+    * apply sa_mul_swapL; [apply sa_mulC; apply uusa_unit; apply empty_1 | apply H0].
+    * apply sa_mulC; apply uusa_unit; apply empty_1.
+  }
+  exists m1; exists m2; exists H1.
+  rewrite Heqm1, Heqm2.
+  clear Heqm1 Heqm2 H1 m1 m2. *)
+  (* And solve the two goals *)
+  rewrite Href; split.
+  * simpl; split; [ apply Hpointsto |].
+    exists (remove (pos, C, f) (get_heap_ptr m)).
+    apply sa_mul_swapL; [apply sa_mulC; apply uusa_unit; apply empty_1 | assumption].
+    (*exists (empty _); apply uusa_unit; apply empty_1.*)
+  * apply HIM.
+Qed.
+
+  
