Java/src/Logic/SpecLogic.v
@@ -1,4 +1,4 @@
-Require Import Later Program ILogic ILEmbed ILInsts.
+Require Import Later Lang Program ILogic ILEmbed ILInsts Maps.
 
 Local Existing Instance ILLaterNat.
 Local Existing Instance ILLaterNatOps.
@@ -35,14 +35,6 @@ Proof.
     * apply IHn. apply Hnat. apply S'. omega.
     * subst. apply S'.
 Defined.
-
-Program Definition prog_spec (X : Prog_wf -> Prop) : spec :=
-  mk_spec (fun (P : Prog_wf) _ => forall (Q : Prog_wf) , Prog_wf_sub P Q -> X Q) _ _.
-Next Obligation.
-  intros; apply H0; etransitivity; eassumption.
-Qed.
-
-Notation "'[prog]' P"    := (prog_spec  P) (at level 65).
 
 Local Existing Instance EmbedILPreDropOp.
 Local Existing Instance EmbedILPreDrop.
