Java/src/Semantics/SemCmdRules.v
@@ -17,7 +17,8 @@ Open Scope open_scope.
     Local Transparent ILLaterNatOps.
     Local Transparent EmbedPSasnSasnOp.
     Local Transparent EmbedILFunDropOp.
-
+    Local Transparent EmbedILFunOp.
+    
 Section Rules.
 
   Section StructuralRules.
@@ -27,13 +28,13 @@ Section Rules.
       (HPost : Q' |-- Q ) :
       {{P'}}c{{Q'}} |-- {{P}}c{{Q}}.
     Proof.
-      intros n Pr Hc Pr' PM m k s h t HPr Hmn Hkm HP; simpl.
-      destruct (Hc _ PM _ _ s h t HPr Hmn Hkm) as [HSafe HQ].
+      intros PM n Pr Hc Pr' m k s h t HPr Hmn Hkm HP; simpl.
+      destruct (Hc _ _ _ s h t HPr Hmn Hkm) as [HSafe HQ].
       + apply HPre; apply HP.
       + split; [apply HSafe|intros t' h' s' H].
         apply HPost. specialize (HQ _ _ _ H). apply HQ.
     Qed.
-
+Local Existing Instance EmbedPSasnSasnOp.
     Definition not_modifies (c : semCmd) (x : var) : Prop :=
       forall PP PM s s' h h' STs STs' n (HSem : c PP PM n s h STs (Some (s', (h', STs')))),
         s x = s' x.
@@ -44,9 +45,9 @@ Section Rules.
       {{ P ** embed R }} c {{ Q ** Exists vs, embed (apply_subst R (subst_fresh vs xs)) }}.
     Proof.
       intros.
-      intros PP n HSpec PP' ? ? ? ? ? ? HPP' Hmn Hkm [h1 [h2 [HSub [HP HR]]]]; split.
+      intros PM PP n HSpec PP' ? ? ? ? ? HPP' Hmn Hkm [h1 [h2 [HSub [HP HR]]]]; split.
       (* safety *)
-      { destruct (HSpec _ PM m k s h STs HPP' Hmn Hkm) as [HS _]; [ | assumption].
+      { destruct (HSpec _ m k s h STs HPP' Hmn Hkm) as [HS _]; [ | assumption].
         solve_model HP. exists h2; apply HSub.
       }
       (* correctness *)
@@ -54,15 +55,15 @@ Section Rules.
       destruct (@cmd_frame c PP' PM s s' h h' h2 h1 k STs STs') as [h'' [HBig Hc]]. 
       + assumption.
       + intros l Hle.
-        destruct (HSpec _ PM m l s h1 STs HPP' Hmn) as [HS _]; [ omega | assumption |].
+        destruct (HSpec _ m l s h1 STs HPP' Hmn) as [HS _]; [ omega | assumption |].
         apply HS.
       + assumption.
-      + destruct (HSpec _ PM m k s h1 STs HPP' Hmn Hkm) as [_ HC]. 
+      + destruct (HSpec _ m k s h1 STs HPP' Hmn Hkm) as [_ HC]. 
         * apply HP.
         * specialize (HC STs' h'' s' Hc).
           exists h'', h2, HBig. split; [assumption |].
           simpl. exists s. unfold apply_subst, id.
-          simpl in HR; unfold id in HR.
+          simpl in HR; unfold id in HR. 
           solve_model HR.
           - apply functional_extensionality. intros x.
             unfold stack_subst, subst_fresh.
@@ -77,8 +78,8 @@ Section Rules.
       (H2 : G |-- {{P2}} c {{Q2}}) :
       G |-- {{P1 //\\ P2}} c {{Q1 //\\ Q2}}.
     Proof.
-      intros n P HPP HG.
-      simpl. intros PM m k s h STs HPP' Hm Hk [HP1 HP2]. split.
+      intros PM n P HPP HG.
+      simpl. intros m k s h STs HPP' Hm Hk [HP1 HP2]. split.
       + eapply H1; eauto.
       + intros STs' h' s' Hsem.
         split; [eapply H1|eapply H2]; eauto.
@@ -99,19 +100,19 @@ Section Rules.
     Lemma seq_rule c1 c2 P Q R :
       ({{P}}c1{{Q}} //\\ {{Q}}c2{{R}}) |-- {{P}}seq_cmd c1 c2{{R}}.
     Proof.
-      intros Pr n [Hc1 Hc2] Pr' PM k m s h STs HPP' Hmn Hkm HP; split.
+      intros PM Pr n [Hc1 Hc2] Pr' k m s h STs HPP' Hmn Hkm HP; split.
       + intros HFail; inversion HFail; subst; clear HFail.	
-        * destruct (Hc1 _ PM _ n0 s h STs HPP' Hmn) as [HS _];
+        * destruct (Hc1 _ _ n0 s h STs HPP' Hmn) as [HS _];
           [omega | assumption | apply HS; assumption ].
-        * destruct (Hc1 _ PM _ n0 s h STs HPP' Hmn) as [_ HC]; [omega | assumption |].
+        * destruct (Hc1 _ _ n0 s h STs HPP' Hmn) as [_ HC]; [omega | assumption |].
           specialize (HC _ _ _ H).
-          destruct (Hc2 _ PM (k - n0) n' s' h' STs' HPP') as [HS _]; [omega | omega | |].
+          destruct (Hc2 _ (k - n0) n' s' h' STs' HPP') as [HS _]; [omega | omega | |].
           apply HC. 
           apply HS; exact H0.
       + intros STs' h' s' HSem; inversion HSem; subst; clear HSem.
-        destruct (Hc1 _ PM _ n0 s h STs HPP' Hmn) as [_ HC1]; [omega | assumption |].
+        destruct (Hc1 _ _ n0 s h STs HPP' Hmn) as [_ HC1]; [omega | assumption |].
         specialize (HC1 _ _ _ H7).
-        destruct (Hc2 _ PM (k - n0) n1 s1 h1 STs1 HPP') as [_ HC2]; [omega | omega | |].
+        destruct (Hc2 _ (k - n0) n1 s1 h1 STs1 HPP') as [_ HC2]; [omega | omega | |].
         apply HC1.
         specialize (HC2 _ _ _ H9).
         solve_model HC2. 
@@ -120,17 +121,17 @@ Section Rules.
     Lemma nondet_rule c1 c2 P Q:
       ({{P}}c1{{Q}} //\\ {{P}}c2{{Q}}) |-- {{P}}nondet_cmd c1 c2{{Q}}.
     Proof.
-      intros n Pr [Hc1 Hc2] Pr' PM k m s h STs HPP' Hmn Hkm HP; split.
+      intros PM n Pr [Hc1 Hc2] Pr' k m s h STs HPP' Hmn Hkm HP; split.
       + intros HFail; inversion HFail; subst; clear HFail.
-        * destruct (Hc1 _ PM _ n0 s h STs HPP' Hmn) as [HS _];
+        * destruct (Hc1 _ _ n0 s h STs HPP' Hmn) as [HS _];
           [omega | assumption | apply HS; assumption].
-        * destruct (Hc2 _ PM _ n0 s h STs HPP' Hmn) as [HS _];
+        * destruct (Hc2 _ _ n0 s h STs HPP' Hmn) as [HS _];
           [omega | assumption | apply HS; assumption].
       + intros h1 s1 STs1 HSem; inversion HSem; subst; clear HSem.
-        * destruct (Hc1 _ PM _ n0 s h STs HPP' Hmn) as [_ HC]; [omega | assumption |].
+        * destruct (Hc1 _ _ n0 s h STs HPP' Hmn) as [_ HC]; [omega | assumption |].
           specialize (HC _ _ _ H6). 
           solve_model HC.
-        * destruct (Hc2 _ PM _ n0 s h STs HPP' Hmn) as [_ HC]; [omega | assumption |].
+        * destruct (Hc2 _ _ n0 s h STs HPP' Hmn) as [_ HC]; [omega | assumption |].
           specialize (HC _ _ _ H6).
           solve_model HC.
     Qed.
@@ -138,21 +139,21 @@ Section Rules.
     Lemma kleene_rule c P:
       {{P}}c{{P}} |-- {{P}} kleene_cmd c {{P}}.
     Proof.
-      intros Pr n Hc Pr' PM m k s h STs HPP' Hmn Hkm Hp; split.
+      intros PM Pr n Hc Pr' m k s h STs HPP' Hmn Hkm Hp; split.
       + intros HFail. generalize dependent m. remember None as cfg.
         induction HFail; intros; inversion Heqcfg; subst.
-        * destruct (Hc _ PM m n0 s h STs HPP' Hmn) as [HS _];
+        * destruct (Hc _ m n0 s h STs HPP' Hmn) as [HS _];
           [omega | assumption | apply HS; assumption].
-        * destruct (Hc _ PM m n0 s h STs HPP' Hmn) as [_ HC]; [omega | assumption |].
-          apply IHHFail with (m-n0); [assumption | reflexivity | omega | omega | ].
+        * destruct (Hc _ m n0 s h STs HPP' Hmn) as [_ HC]; [omega | assumption |].
+          apply IHHFail with (m-n0); [assumption | assumption| reflexivity | omega | omega | ].
           specialize (HC _ _ _ H).
           solve_model HC.
       + intros. remember (Some (s', (h', STs'))) as cfg. generalize dependent m. 
         induction H; inversion Heqcfg; subst; intros.
         * solve_model Hp.
-        * destruct (Hc _ PM m n0 s h STs HPP' Hmn) as [_ HC]; [omega | assumption |].
+        * destruct (Hc _ m n0 s h STs HPP' Hmn) as [_ HC]; [omega | assumption |].
           specialize (HC _ _ _ H).
-          assert ((((P PM STs' s') Pr0) ((m - n0) - n1)) h') as H2. 
+          assert ((((P s' PM STs') Pr0) ((m - n0) - n1)) h') as H2. 
             apply IHkleene_sem; try assumption; try omega. 
           solve_model H2.
     Qed.
@@ -160,7 +161,7 @@ Section Rules.
     Lemma assume_rule P (t : vlogic) :
       |-- {{P}} assume_cmd t {{t /\\ P}}.
     Proof.
-      intros n Pr Hc Pr' PM m k s h STs HPP' Hmn Hkm Hp; split.
+      intros PM n Pr Hc Pr' m k s h STs HPP' Hmn Hkm Hp; split.
       + intros HFail. inversion HFail.
       + intros STs' h' s' H. remember (Some (s', (h', STs'))) as cfg; induction H.
         inversion Heqcfg; subst; intros.
@@ -170,7 +171,7 @@ Section Rules.
     Lemma assert_rule (P : psasn) (p : vlogic) (HPe : P |-- embed p) :
       |-- {{P}} assert_cmd p {{P}}.
     Proof.
-      intros n Pr Hc Pr' PM m k s h STs HPP' Hmn Hkm Hp; specialize (HPe _ _ _ _ _ _ Hp); split.
+      intros PM n Pr Hc Pr' m k s h STs HPP' Hmn Hkm Hp; specialize (HPe _ _ _ _ _ _ Hp); split.
       + intros HF; inversion HF; subst; auto.
       + intros STs' h' s' HSem; inversion HSem; subst.
         solve_model Hp.
@@ -182,27 +183,27 @@ Section Rules.
     (Forall x, {{P x}} c {{q}}) -|- {{Exists x, P x}} c {{q}}.
   Proof.
   	split.
-  	+ intros n Pr Hp Pr' PM m k s h STs HPP' Hmn Hkm [x Hxp]; specialize (Hp x); auto.
-  	+ intros n Pr Hp x Pr' PM m k s h STs HPP' Hmn Hkm Hxp.
+  	+ intros PM n Pr Hp Pr' m k s h STs HPP' Hmn Hkm [x Hxp]; specialize (Hp x); auto.
+  	+ intros PM n Pr Hp x Pr' m k s h STs HPP' Hmn Hkm Hxp.
   	  apply Hp; try assumption. exists x; apply Hxp.
   Qed.
 
   (* Holds only in one direction unless annotations on assertion logic, which is ugly - well, it's happened. - F.
      This is the important direction, though *)
-  Lemma I_precond (SP : spec) (P Q : psasn) c:
+  Lemma I_precond (SP : pspec) (P Q : psasn) c:
     (SP -->> {{ P }} c {{ Q }}) -|- {{ SP /\\  P }} c {{ Q }}.
   Proof.
   	split.
-  	+ intros Pr n Hp Pr' PM m k s h STs HPP' Hmn Hkm [HSP HP].
+  	+ intros PM Pr n Hp Pr' m k s h STs HPP' Hmn Hkm [HSP HP].
   	  specialize (Hp Pr' HPP' m Hmn HSP).
   	  apply Hp; reflexivity || assumption.
-  	+ intros Pr n Hp Pr' HPP' m Hnm HSP Pr'' PM k l s h STs HPP'' Hkm Hkl HP.
+  	+ intros PM Pr n Hp Pr' HPP' m Hnm HSP Pr'' k l s h STs HPP'' Hkm Hkl HP.
   	  apply Hp.
   	  * transitivity Pr'; assumption.
   	  * omega.
   	  * omega.
   	  * simpl. split. 
-        assert ((SP Pr'') k). solve_model HSP. intros a b. simpl. intuition.
+        assert ((SP PM Pr'') k). solve_model HSP. intros a b. simpl. intuition.
         apply H. apply HP.
   Qed.
 
